Graveyard.v
@@ -1,4 +1,6 @@
 Require Import Arith Lia.
+Require Import List. Import ListNotations.
+
 
 
 (* This is the current contender for largest number. *)
@@ -304,4 +306,825 @@ Proof.
       -- apply (geS_ack 5 42); lia.
       -- apply H.
   - apply (geS_ack 4 42); lia.
+Qed.
+
+Fixpoint iter (f : nat -> nat) (b : nat) :=
+  match b with
+  | 0 => 1
+  | S b' => f (iter f b')
+  end.
+
+Fixpoint ack (n a b : nat) :=
+  match n with
+  | 0 => S b
+  | 1 => a + b
+  | S n' => iter (ack n' a) b
+  end.
+
+
+(* This is the previous contender for largest number *)
+(* Submitted by codyroux *)
+Definition contender_4 := ack 5 42 10002.
+
+
+(* Definition of the language STLC+NatRec: *)
+
+Inductive type :=
+| tpNat: type
+| tpArr: type -> type -> type.
+
+Fixpoint type_eqb(t1 t2: type): bool :=
+  match t1, t2 with
+  | tpNat, tpNat => true
+  | tpArr A B, tpArr C D => andb (type_eqb A C) (type_eqb B D)
+  | _, _ => false
+  end.
+
+Fixpoint type_depth(t: type): nat :=
+  match t with
+  | tpNat => 1
+  | tpArr t1 t2 => S (max (type_depth t1) (type_depth t2))
+  end.
+
+Fixpoint interp_type(tp: type): Type :=
+  match tp with
+  | tpNat => nat
+  | tpArr t1 t2 => (interp_type t1) -> (interp_type t2)
+  end.
+
+Inductive term :=
+| tVar(x: nat) (* 0 = last element of the env, ie the outermost binder (reversed DeBruijn) *)
+| tLam(A B: type)(body: term)
+| tApp(t1 t2: term)
+| tO
+| tS
+| tNatRec(R: type).
+
+Definition nat_depth(n: nat) := S n.
+
+Fixpoint term_depth(t: term): nat :=
+  match t with
+  | tVar x => S (nat_depth x)
+  | tLam A B body => S (max (max (type_depth A) (type_depth B)) (term_depth body))
+  | tApp t1 t2 => S (max (term_depth t1) (term_depth t2))
+  | tO => 1
+  | tS => 1
+  | tNatRec R => S (type_depth R)
+  end.
+
+Definition lookup{T}(e: list T)(n: nat): option T :=
+  let l := List.length e in if l <=? n then None else nth_error e (l - S n).
+
+Goal lookup [10; 11; 12] 0 = Some 12. reflexivity. Qed.
+Goal lookup [10; 11; 12] 1 = Some 11. reflexivity. Qed.
+Goal lookup [10; 11; 12] 2 = Some 10. reflexivity. Qed.
+Goal lookup [10; 11; 12] 3 = None. reflexivity. Qed.
+
+Definition error{tp: type}: interp_type tp.
+  revert tp.
+  refine (fix rec tp := _).
+  destruct tp; simpl.
+  - exact 0.
+  - intros _. apply rec.
+Defined.
+
+Definition cast_error(from to: type):
+  ((interp_type from -> interp_type to) * (interp_type to -> interp_type from)).
+  split; intros; exact error.
+Defined.
+
+Definition cast_impl(from to: type):
+  ((interp_type from -> interp_type to) * (interp_type to -> interp_type from)).
+  revert from to.
+  induction from; intros; simpl in *.
+  - destruct to; simpl.
+    + split; exact id.
+    + exact (cast_error tpNat (tpArr to1 to2)).
+  - destruct to.
+    + exact (cast_error (tpArr from1 from2) tpNat).
+    + destruct (type_eqb from1 to1) eqn: E1;
+      destruct (type_eqb from2 to2) eqn: E2;
+      simpl in *.
+      {
+        specialize (IHfrom1 to1).
+        specialize (IHfrom2 to2).
+        destruct IHfrom1 as [F1T1 T1F1].
+        destruct IHfrom2 as [F2T2 T2F2].
+        split.
+        * intros F arg. apply F2T2. apply F. apply T1F1. apply arg.
+        * intros F arg. apply T2F2. apply F. apply F1T1. apply arg.
+      }
+      all: exact (cast_error (tpArr from1 from2) (tpArr to1 to2)).
+Defined.
+
+(* designed to be computable (no opaque proofs) *)
+Definition cast{from: type}(to: type): interp_type from -> interp_type to :=
+  fst (cast_impl from to).
+
+Definition interp_term: forall (e: list {tp: type & interp_type tp}) (t: term),
+    {tp: type & interp_type tp}.
+  refine (fix rec e t {struct t} :=
+  match t with
+  | tVar x => _
+  | tLam A B body => _
+  | tApp t1 t2 => _
+  | tO => _
+  | tS => _
+  | tNatRec R => _
+  end).
+  - destruct (lookup e x) as [R|].
+    + exact R.
+    + exact (existT _ tpNat error).
+  - refine (existT _ (tpArr A B) _).
+    simpl.
+    intro x'.
+    set (r := (projT2 (rec ((existT _ A x') :: e) body))).
+    simpl in r.
+    exact (cast B r).
+  - destruct (rec e t1) as [R1 r1] eqn: E1.
+    destruct (rec e t2) as [R2 r2] eqn: E2.
+    destruct R1 as [|A B]; [exact (existT _ tpNat error)|].
+    simpl in *.
+    exact (existT _ _ (r1 (cast A r2))).
+  - exact (existT _ tpNat 0).
+  - exact (existT _ (tpArr tpNat tpNat) S).
+  - set (r := (@Nat.recursion (interp_type R))).
+    exact (existT _ (tpArr R (tpArr (tpArr tpNat (tpArr R R)) (tpArr tpNat R))) r).
+Defined.
+
+
+(* Defining the new contender: *)
+
+Fixpoint typesUpTo(n: nat): list type :=
+  match n with
+  | O => []
+  | S m =>
+    let r := typesUpTo m in
+    tpNat :: List.map (fun '(t1, t2) => tpArr t1 t2) (list_prod r r)
+  end.
+
+Lemma typesUpTo_correct: forall n t,
+    type_depth t <= n <-> List.In t (typesUpTo n).
+Proof.
+  induction n; intros; split; intros.
+  - destruct t; simpl in *; lia.
+  - simpl in *. contradiction.
+  - simpl. destruct t; [auto|].
+    right. simpl in *.
+    match goal with
+    | |- In ?e (map ?f _) => change e with (f (t1, t2))
+    end.
+    apply in_map.
+    apply in_prod; eapply IHn; lia.
+  - simpl in *. destruct H.
+    + subst. simpl. lia.
+    + apply in_map_iff in H.
+      destruct H as [[t1 t2] [? H]].
+      subst t.
+      apply in_prod_iff in H.
+      destruct H as [H1 H2].
+      pose proof ((proj2 (IHn _)) H1).
+      pose proof ((proj2 (IHn _)) H2).
+      simpl.
+      lia.
+Qed.
+
+Fixpoint natsUpTo(n: nat): list nat :=
+  match n with
+  | O => []
+  | S m => m :: natsUpTo m
+  end.
+
+Lemma natsUpTo_correct: forall n m,
+    nat_depth m <= n <-> List.In m (natsUpTo n).
+Proof.
+  induction n; intros; unfold nat_depth in *; split; intros; simpl in *.
+  - exfalso. lia.
+  - contradiction.
+  - assert (n = m \/ S m <= n) as C by lia. destruct C as [C | C]; firstorder idtac.
+  - destruct H.
+    + lia.
+    + specialize (IHn m). apply proj2 in IHn. specialize (IHn H). lia.
+Qed.
+
+Fixpoint termsUpTo(n: nat): list term :=
+  match n with
+  | O => []
+  | S m =>
+    List.map tVar (natsUpTo m) ++
+    List.map (fun '(A, B, body) => tLam A B body)
+             (list_prod (list_prod (typesUpTo m) (typesUpTo m)) (termsUpTo m)) ++
+    List.map (fun '(t1, t2) => tApp t1 t2)
+             (list_prod (termsUpTo m) (termsUpTo m)) ++
+    [tO] ++ [tS] ++
+    List.map tNatRec (typesUpTo m)
+  end.
+
+Lemma termsUpTo_correct: forall n t,
+    term_depth t <= n <-> List.In t (termsUpTo n).
+Proof.
+  induction n; intros; split; intros.
+  - destruct t; simpl in *; lia.
+  - simpl in *. contradiction.
+  - destruct t; simpl in *.
+    + do 0 (apply in_or_app; right). apply in_or_app; left.
+      apply in_map. apply natsUpTo_correct. lia.
+    + do 1 (apply in_or_app; right). apply in_or_app; left.
+      match goal with
+      | |- In ?e (map ?f _) => change e with (f (A, B, t))
+      end.
+      repeat first
+             [ apply in_map
+             | apply in_prod
+             | apply (proj1 (natsUpTo_correct _ _))
+             | apply (proj1 (typesUpTo_correct _ _))
+             | apply (proj1 (IHn _))
+             | lia].
+    + do 2 (apply in_or_app; right). apply in_or_app; left.
+      match goal with
+      | |- In ?e (map ?f _) => change e with (f (t1, t2))
+      end.
+      repeat first
+             [ apply in_map
+             | apply in_prod
+             | apply (proj1 (natsUpTo_correct _ _))
+             | apply (proj1 (typesUpTo_correct _ _))
+             | apply (proj1 (IHn _))
+             | lia].
+    + do 3 (apply in_or_app; right). simpl. auto.
+    + do 3 (apply in_or_app; right). simpl. auto.
+    + do 3 (apply in_or_app; right). simpl. right. right.
+      repeat first
+             [ apply in_map
+             | apply in_prod
+             | apply (proj1 (natsUpTo_correct _ _))
+             | apply (proj1 (typesUpTo_correct _ _))
+             | apply (proj1 (IHn _))
+             | lia].
+  - simpl in *.
+    repeat ((simpl in H || apply in_app_iff in H || idtac); destruct H).
+    + apply in_map_iff in H.
+      destruct H as [x [? H]].
+      subst t.
+      pose proof ((proj2 (natsUpTo_correct _ _)) H).
+      simpl.
+      lia.
+    + apply in_map_iff in H.
+      destruct H as [[[A B] body] [? H]].
+      subst t.
+      repeat (apply in_prod_iff in H; destruct H).
+      pose proof ((proj2 (typesUpTo_correct _ _)) H).
+      pose proof ((proj2 (typesUpTo_correct _ _)) H1).
+      pose proof ((proj2 (IHn _)) H0).
+      simpl.
+      lia.
+    + apply in_map_iff in H.
+      destruct H as [[t1 t2] [? H]].
+      subst t.
+      repeat (apply in_prod_iff in H; destruct H).
+      pose proof ((proj2 (IHn _)) H).
+      pose proof ((proj2 (IHn _)) H0).
+      simpl.
+      lia.
+    + simpl. lia.
+    + simpl. lia.
+    + apply in_map_iff in H.
+      destruct H as [R [? H]].
+      subst t.
+      pose proof ((proj2 (typesUpTo_correct _ _)) H).
+      simpl.
+      lia.
+Qed.
+
+Definition eval(t : term): nat :=
+  let (tp, res) := interp_term nil t in
+  match tp as t0 return (interp_type t0 -> nat) with
+  | tpNat         => fun (res: interp_type tpNat) => res
+  | tpArr tp1 tp2 => fun (res: interp_type (tpArr tp1 tp2)) => 0
+  end res.
+
+Fixpoint maxBy{T: Type}(f: T -> nat)(currentMax: nat)(currentBest: T)(l: list T): T :=
+  match l with
+  | nil => currentBest
+  | cons h t =>
+    if currentMax <? (f h) then
+      maxBy f (f h) h t
+    else
+      maxBy f currentMax currentBest t
+  end.
+
+Definition largest_of_depth(n: nat): term := maxBy eval 0 tO (termsUpTo n).
+
+Eval vm_compute in (largest_of_depth 1).
+Eval vm_compute in (largest_of_depth 2).
+Eval vm_compute in (largest_of_depth 3).
+Eval vm_compute in (largest_of_depth 4).
+
+Definition largest_STLCNatRec_nat_of_depth(n: nat): nat := eval (largest_of_depth n).
+
+(* Small examples are computable: *)
+Eval vm_compute in (largest_STLCNatRec_nat_of_depth 1).
+Eval vm_compute in (largest_STLCNatRec_nat_of_depth 2).
+Eval vm_compute in (largest_STLCNatRec_nat_of_depth 3).
+Eval vm_compute in (largest_STLCNatRec_nat_of_depth 4).
+(* but as soon as it would get interesting, it becomes too inefficient *)
+
+
+(* This is the current contender for largest number *)
+(* Submitted by samuelgruetter *)
+(* <brag>Note how its definition does not require any large literals</brag> ;-) *)
+Definition contender_5: nat := largest_STLCNatRec_nat_of_depth 42.
+
+
+(* Reification automation: *)
+
+Definition type_eq_dec: forall x y : type, {x = y} + {x <> y}.
+  induction x; destruct y eqn: E; intros; simpl.
+  - left. reflexivity.
+  - right. intro C. discriminate.
+  - right. intro C. discriminate.
+  - specialize (IHx1 t1).
+    specialize (IHx2 t2).
+    destruct IHx1 as [E1 | N1]; destruct IHx2 as [E2 | N2]; try (right; congruence).
+    left. subst. reflexivity.
+Defined.
+
+Lemma type_eqb_true: forall t1 t2, type_eqb t1 t2 = true -> t1 = t2.
+Proof.
+  induction t1; intros; destruct t2; simpl in *; try congruence.
+  apply Bool.andb_true_iff in H. destruct H. f_equal; eauto.
+Qed.
+
+Lemma type_eqb_same: forall t, type_eqb t t = true.
+Proof.
+  induction t; simpl.
+  - reflexivity.
+  - rewrite IHt1, IHt2. reflexivity.
+Qed.
+
+(* only for the reification machinery, will not show up in the final proof *)
+Require Import FunctionalExtensionality.
+
+Lemma cast_impl_same: forall (B: type) (t: interp_type B),
+    fst (cast_impl B B) t = t /\ snd (cast_impl B B) t = t.
+Proof.
+  induction B; intros; simpl; unfold id.
+  - auto.
+  - do 2 rewrite type_eqb_same.
+    destruct (cast_impl B1 B1) as [fw1 bw1] eqn: E1.
+    destruct (cast_impl B2 B2) as [fw2 bw2] eqn: E2.
+    simpl in *.
+    split; extensionality arg.
+    + specialize (IHB1 arg).
+      apply proj2 in IHB1.
+      rewrite IHB1.
+      specialize (IHB2 (t arg)).
+      apply proj1 in IHB2.
+      exact IHB2.
+    + specialize (IHB1 arg).
+      apply proj1 in IHB1.
+      rewrite IHB1.
+      specialize (IHB2 (t arg)).
+      apply proj2 in IHB2.
+      exact IHB2.
+Qed.
+
+Lemma cast_same: forall (B: type) (t: interp_type B),
+    cast B t = t.
+Proof.
+  intros. unfold cast.
+  pose proof (cast_impl_same B t) as P.
+  apply proj1 in P.
+  exact P.
+Qed.
+
+Lemma interp_tVar: forall e x (p: {tp: type & interp_type tp}),
+    lookup e x = Some p ->
+    interp_term e (tVar x) = p.
+Proof. intros. simpl. rewrite H. reflexivity. Qed.
+
+Lemma interp_tVar_head: forall e y (p: {tp: type & interp_type tp}),
+    y = List.length e ->
+    interp_term (p :: e) (tVar y) = p.
+Proof.
+  intros. subst. simpl. unfold lookup, List.find.
+  change (length (p :: e)) with (S (length e)).
+  destruct (S (length e) <=? length e) eqn: E. {
+    apply Nat.leb_le in E. exfalso. lia.
+  }
+  rewrite Nat.sub_diag.
+  reflexivity.
+Qed.
+
+Lemma interp_tVar_tail: forall e y (p1 p2: {tp: type & interp_type tp}),
+    length e <=? y = false ->
+    interp_term e (tVar y) = p2 ->
+    interp_term (p1 :: e) (tVar y) = p2.
+Proof.
+  intros. simpl in *. unfold lookup, List.find in *.
+  change (length (p1 :: e)) with (S (length e)).
+  rewrite H in H0.
+  apply Nat.leb_gt in H.
+  replace (S (length e) - S y) with (S (length e - S y)) by lia.
+  destruct (S (length e) <=? y) eqn: E. {
+    apply Nat.leb_le in E. exfalso. lia.
+  }
+  simpl.
+  assumption.
+Qed.
+
+Lemma interp_tLam: forall e A B body f,
+  (forall x0, interp_term (existT interp_type A x0 :: e) body = existT _ B (f x0)) ->
+  interp_term e (tLam A B body) = existT _ (tpArr A B) f.
+Proof.
+  simpl.
+  intros.
+  f_equal.
+  extensionality x'.
+  specialize (H x').
+  destruct (interp_term (existT interp_type A x' :: e) body) eqn: E.
+  inversion H.
+  subst.
+  simpl.
+  apply cast_same.
+Qed.
+
+Lemma interp_tApp: forall e t1 t2 A B (f: interp_type A -> interp_type B) (a: interp_type A),
+    interp_term e t1 = existT _ (tpArr A B) f ->
+    interp_term e t2 = existT _ A a ->
+    interp_term e (tApp t1 t2) = existT _ B (f a).
+Proof.
+  intros.
+  simpl.
+  destruct (interp_term e t1) eqn: E1.
+  destruct (interp_term e t2) eqn: E2.
+  pose proof (EqdepFacts.eq_sigT_fst H). subst x.
+  apply Eqdep_dec.inj_pair2_eq_dec in H. 2: apply type_eq_dec. subst i.
+  pose proof (EqdepFacts.eq_sigT_fst H0). subst x0.
+  apply Eqdep_dec.inj_pair2_eq_dec in H0. 2: apply type_eq_dec. subst i0.
+  rewrite cast_same.
+  reflexivity.
+Qed.
+
+Lemma interp_tO: forall e, interp_term e tO = existT _ tpNat 0.
+Proof. intros. reflexivity. Qed.
+
+Lemma interp_tS: forall e, interp_term e tS = existT _ (tpArr tpNat tpNat) S.
+Proof. intros. reflexivity. Qed.
+
+Lemma interp_tNatRec: forall e R,
+    interp_term e (tNatRec R) =
+    existT _ (tpArr R (tpArr (tpArr tpNat (tpArr R R)) (tpArr tpNat R)))
+           (@Nat.recursion (interp_type R)).
+Proof.
+  intros. subst. reflexivity.
+Qed.
+
+(*
+Notation "A --> B" := (tpArr A B) (at level 60, right associativity).
+*)
+
+Ltac reify_type T :=
+  lazymatch T with
+  | ?A -> ?B => let A' := reify_type A in
+                let B' := reify_type B in
+                constr:(tpArr A' B')
+  | nat => constr:(tpNat)
+  | interp_type ?A => constr:(A)
+  | _ => fail "" T "is not a type"
+  end.
+
+Ltac t :=
+  lazymatch goal with
+  | |- interp_term ?e ?t = existT _ ?T (fun _ => _) =>
+    eapply interp_tLam; intros ?
+  | |- interp_term ?e ?t = existT _ ?T O =>
+    eapply interp_tO
+  | |- interp_term ?e ?t = existT _ ?T S =>
+    eapply interp_tS
+  | |- interp_term ?e ?t = existT _ ?T Nat.recursion =>
+    eapply interp_tNatRec
+  | |- interp_term ?e ?t = existT _ ?B (?f ?a) =>
+    let A := type of a in
+    let A := eval cbv beta iota in A in
+    let A := reify_type A in
+    eapply (interp_tApp e _ _ A B)
+  | |- interp_term ?e ?t = existT _ ?T ?x =>
+    is_var x;
+    first [ eapply interp_tVar_head; cbv [length]; reflexivity
+          | eapply interp_tVar_tail; cbv [length]]
+  end.
+
+
+(* Expressing contender_4 as an STLC+NatRec term: *)
+
+Definition ack'(n: nat): nat -> nat -> nat :=
+  Nat.recursion
+    (fun a b => S b)
+    (fun (pred0: nat) (rec0: nat -> nat -> nat) =>
+       Nat.recursion
+         (Nat.recursion (fun (m: nat) => m)
+                        (fun (pred: nat) (rec: nat -> nat) (m: nat) => S (rec m)))
+         (fun (pred: nat) (rec: nat -> nat -> nat) =>
+            (fun a b => Nat.recursion 1 (fun pred1 rec1 => rec a rec1) b))
+         pred0)
+    n.
+
+Lemma iter_proper: forall f1 f2,
+    (forall x, f1 x = f2 x) ->
+    forall b, iter f1 b = iter f2 b.
+Proof.
+  induction b.
+  - reflexivity.
+  - simpl. rewrite IHb. apply H.
+Qed.
+
+Definition iter' (f : nat -> nat) : nat -> nat :=
+  Nat.recursion 1 (fun (pred: nat) (rec: nat) => f rec).
+
+Lemma iter'_equiv: forall f b, iter' f b = iter f b.
+Proof. induction b; intros; simpl; congruence. Qed.
+
+Definition add': nat -> nat -> nat :=
+  Nat.recursion (fun (m: nat) => m) (fun (pred: nat) (rec: nat -> nat) (m: nat) => S (rec m)).
+
+Lemma add'_equiv: forall n m, add' n m = Nat.add n m.
+Proof.
+  induction n; intros; simpl.
+  - reflexivity.
+  - rewrite <- IHn. reflexivity.
+Qed.
+
+Definition mul': nat -> nat -> nat :=
+  Nat.recursion (fun (m: nat) => 0)
+                (fun (pred: nat) (rec: nat -> nat) (m: nat) => add' m (rec m)).
+
+Lemma mul'_equiv: forall n m, mul' n m = Nat.mul n m.
+Proof.
+  induction n; intros; simpl.
+  - reflexivity.
+  - rewrite <- IHn. rewrite add'_equiv. reflexivity.
+Qed.
+
+Definition pow'(n: nat): nat -> nat :=
+  Nat.recursion 1 (fun (pred: nat) (rec: nat) => mul' n rec).
+
+Lemma pow'_equiv: forall n m, pow' n m = Nat.pow n m.
+Proof.
+  induction m; intros; simpl.
+  - reflexivity.
+  - rewrite <- IHm. rewrite mul'_equiv. reflexivity.
+Qed.
+
+Lemma ack'_equiv: forall n a b, ack' n a b = ack n a b.
+Proof.
+  induction n; intros; simpl.
+  - reflexivity.
+  - destruct n.
+    + simpl. apply add'_equiv.
+    + specialize (IHn a).
+      rewrite <- (iter_proper _ _ IHn).
+      rewrite <- iter'_equiv. reflexivity.
+Qed.
+
+Lemma ack'_reification_helper: exists res,
+    interp_term nil res
+    = existT _ (tpArr tpNat (tpArr tpNat (tpArr tpNat tpNat))) ack'.
+Proof.
+  eexists.
+  unfold ack'.
+  repeat t.
+  all: reflexivity.
+Defined.
+
+Definition ack_reified: term.
+  let r := eval unfold ack'_reification_helper in ack'_reification_helper in
+  match r with
+  | ex_intro _ ?x _ => exact x
+  end.
+Defined.
+
+Lemma interp_ack_reified: projT2 (interp_term nil ack_reified) = ack'.
+Proof. reflexivity. Qed.
+
+Eval cbv in (term_depth ack_reified).
+
+Definition contender_4': nat.
+  let r := eval unfold pow', mul', add' in (ack' 5 (mul' 6 7) (S (S (pow' 10 4)))) in exact r.
+Defined.
+
+Lemma f_equal_ack'_equiv: forall n a b1 b2 : nat,
+    b1 = b2 ->
+    ack' n a b1 = ack n a b2.
+Proof.
+  intros.
+  rewrite ack'_equiv.
+  f_equal.
+  assumption.
+Qed.
+
+Lemma contender_4'_equiv: contender_4' = contender_4.
+Proof.
+  unfold contender_4', contender_4.
+  apply f_equal_ack'_equiv.
+  vm_compute.
+  reflexivity.
+Qed.
+
+Definition contender_4'': nat.
+  let r := eval unfold contender_4', ack' in contender_4' in exact r.
+Defined.
+
+Lemma contender_4''_equiv: contender_4'' = contender_4.
+Proof.
+  etransitivity. 2: exact contender_4'_equiv.
+  unfold contender_4'', contender_4'.
+  unfold ack'.
+  repeat apply f_equal.
+  reflexivity.
+Qed.
+
+Lemma contender_4''_reification_helper: exists res,
+    interp_term nil res
+    = existT _ tpNat contender_4''.
+Proof.
+  eexists.
+  unfold contender_4''.
+  repeat t.
+  all: reflexivity.
+Defined.
+
+Definition contender_4''_reified: term.
+  let r := eval unfold contender_4''_reification_helper in contender_4''_reification_helper in
+  match r with
+  | ex_intro _ ?x _ => exact x
+  end.
+Defined.
+
+Lemma interp_contender_4''_reified:
+  projT2 (interp_term nil contender_4''_reified) = contender_4''.
+Proof.
+  cbv -[Nat.recursion].
+  repeat apply f_equal.
+  reflexivity.
+Qed.
+
+Lemma eval_contender_4''_reified:
+  eval contender_4''_reified = contender_4''.
+Proof.
+  unfold eval.
+  cbv -[Nat.recursion].
+  repeat apply f_equal.
+  reflexivity.
+Qed.
+
+Eval cbv in (term_depth contender_4''_reified).
+
+
+(* Proving that the new contender is bigger than the previous one: *)
+
+Lemma maxBy_In{T: Type}: forall f (l: list T) currentMax currentBest,
+    currentMax = f currentBest ->
+    List.In (maxBy f currentMax currentBest l) l \/ maxBy f currentMax currentBest l = currentBest.
+Proof.
+  induction l; intros.
+  - simpl. auto.
+  - subst. simpl in *.
+    destruct (f currentBest <? f a) eqn: E.
+    + specialize (IHl (f a) _ eq_refl). firstorder congruence.
+    + specialize (IHl (f currentBest) _ eq_refl). firstorder congruence.
+Qed.
+
+Lemma maxBy_at_least_currentMax{T: Type}: forall (f: T -> nat) l currentMax currentBest,
+    f currentBest = currentMax ->
+    currentMax <= f (maxBy f currentMax currentBest l).
+Proof.
+  induction l; intros; simpl in *.
+  - lia.
+  - subst. destruct (f currentBest <? f a) eqn: E.
+    + apply Nat.ltb_lt in E.
+      specialize (IHl (f a) _ eq_refl).
+      lia.
+    + apply Nat.ltb_ge in E.
+      eapply IHl.
+      reflexivity.
+Qed.
+
+Lemma lowerbound_maxBy{T: Type}: forall (f: T -> nat) x l currentMax currentBest,
+    List.In x l ->
+    f currentBest = currentMax ->
+    f x <= f (maxBy f currentMax currentBest l).
+Proof.
+  induction l; intros; simpl in *.
+  - contradiction.
+  - destruct H.
+    + subst.
+      destruct (f currentBest <? f x) eqn: E.
+      * apply Nat.ltb_lt in E.
+        eapply maxBy_at_least_currentMax.
+        reflexivity.
+      * apply Nat.ltb_ge in E.
+        eapply Nat.le_trans. 1: eassumption.
+        eapply maxBy_at_least_currentMax.
+        reflexivity.
+    + subst.
+      destruct (f currentBest <? f a) eqn: E.
+      * apply Nat.ltb_lt in E.
+        eauto.
+      * apply Nat.ltb_ge in E.
+        eauto.
+Qed.
+
+Lemma upperbound_eval: forall t,
+    eval t <= eval (largest_of_depth (term_depth t)).
+Proof.
+  intros. unfold largest_of_depth.
+  eapply Nat.le_trans. 2: {
+    eapply lowerbound_maxBy with (x := t). 2: reflexivity.
+    eapply termsUpTo_correct.
+    lia.
+  }
+  lia.
+Qed.
+
+Lemma maxBy_monotone{T: Type}: forall f (l1 l2: list T) currentMax currentBest,
+    (forall x, In x l1 -> In x l2) ->
+    f currentBest = currentMax ->
+    f (maxBy f currentMax currentBest l1) <= f (maxBy f currentMax currentBest l2).
+Proof.
+  intros. subst.
+  pose proof (maxBy_In f l1 (f currentBest) _ eq_refl) as P.
+  destruct P as [P | P].
+  - specialize (H _ P).
+    eapply lowerbound_maxBy. 1: exact H. reflexivity.
+  - rewrite P. eapply maxBy_at_least_currentMax. reflexivity.
+Qed.
+
+Lemma largest_of_depth_monotone: forall n1 n2,
+    n1 <= n2 ->
+    eval (largest_of_depth n1) <= eval (largest_of_depth n2).
+Proof.
+  intros.
+  unfold largest_of_depth.
+  eapply (maxBy_monotone eval (termsUpTo n1) (termsUpTo n2)). 2: reflexivity.
+  intros.
+  eapply termsUpTo_correct.
+  eapply termsUpTo_correct in H0.
+  eapply Nat.le_trans; eassumption.
+Qed.
+
+Lemma largest_of_depth_strictly_monotone: forall n1 n2,
+    0 < n1 < n2 ->
+    eval (largest_of_depth n1) < eval (largest_of_depth n2).
+Proof.
+  intros.
+  unfold largest_of_depth.
+  destruct n2 as [|n2]. 1: exfalso; lia.
+  simpl.
+  eapply Nat.le_lt_trans. 1: eapply largest_of_depth_monotone with (n2 := n2). 1: lia.
+  unfold largest_of_depth.
+  eapply Nat.lt_le_trans. 2: {
+    eapply lowerbound_maxBy with (x := (tApp tS (maxBy eval 0 tO (termsUpTo n2)))).
+    2: reflexivity.
+    apply in_app_iff; right.
+    apply in_app_iff; right.
+    apply in_app_iff; left.
+    match goal with
+    | |- In (tApp ?t1 ?t2) (map _ _) =>
+      change (tApp t1 t2) with ((fun '(t10, t20) => tApp t10 t20) (t1, t2))
+    end.
+    eapply in_map.
+    apply in_prod.
+    - destruct n2 as [|n2]. 1: exfalso; lia.
+      simpl.
+      do 3 (apply in_app_iff; right).
+      simpl. auto.
+    - pose proof (maxBy_In eval (termsUpTo n2) 0 tO eq_refl) as P.
+      destruct P as [P | P].
+      + exact P.
+      + rewrite P.
+        destruct n2 as [|n2]. 1: exfalso; lia.
+        simpl.
+        do 3 (apply in_app_iff; right).
+        simpl. auto.
+  }
+  generalize (maxBy eval 0 tO (termsUpTo n2)). intro t.
+  unfold eval.
+  simpl.
+  destruct (interp_term [] t) as [tp1 r1] eqn: E1.
+  destruct tp1 as [|A1 B1].
+  - unfold cast, cast_impl. simpl. unfold id. lia.
+  - lia.
+Qed.
+
+Theorem contender_4_lt_contender_5 : contender_4 < contender_5.
+Proof.
+  rewrite <- contender_4''_equiv.
+  rewrite <- eval_contender_4''_reified.
+  unfold contender_5, largest_STLCNatRec_nat_of_depth.
+  eapply Nat.le_lt_trans.
+  - eapply upperbound_eval.
+  - eapply largest_of_depth_strictly_monotone.
+    cbv.
+    lia.
 Qed.
